DynamoDbEncryption/runtimes/java/src/main/smithy-generated/software/amazon/cryptography/dbencryptionsdk/dynamodb/json/model/EncryptObjectOutput.java
@@ -13,7 +13,7 @@ public class EncryptObjectOutput {
   /**
    * The encrypted JSON object.
    */
-  private final String encryptedObject;
+  private final Json encryptedObject;
 
   /**
    * A parsed version of the header written with the encrypted JSON object.
@@ -28,7 +28,7 @@ public class EncryptObjectOutput {
   /**
    * @return The encrypted JSON object.
    */
-  public String encryptedObject() {
+  public Json encryptedObject() {
     return this.encryptedObject;
   }
 
@@ -51,12 +51,12 @@ public class EncryptObjectOutput {
     /**
      * @param encryptedObject The encrypted JSON object.
      */
-    Builder encryptedObject(String encryptedObject);
+    Builder encryptedObject(Json encryptedObject);
 
     /**
      * @return The encrypted JSON object.
      */
-    String encryptedObject();
+    Json encryptedObject();
 
     /**
      * @param parsedHeader A parsed version of the header written with the encrypted JSON object.
@@ -73,7 +73,7 @@ public class EncryptObjectOutput {
 
   static class BuilderImpl implements Builder {
 
-    protected String encryptedObject;
+    protected Json encryptedObject;
 
     protected ParsedHeader parsedHeader;
 
@@ -84,12 +84,12 @@ public class EncryptObjectOutput {
       this.parsedHeader = model.parsedHeader();
     }
 
-    public Builder encryptedObject(String encryptedObject) {
+    public Builder encryptedObject(Json encryptedObject) {
       this.encryptedObject = encryptedObject;
       return this;
     }
 
-    public String encryptedObject() {
+    public Json encryptedObject() {
       return this.encryptedObject;
     }
 
