DynamoDbEncryption/runtimes/java/src/main/smithy-generated/software/amazon/cryptography/dbencryptionsdk/dynamodb/json/model/Json.java
@@ -1,0 +1,101 @@
+// Copyright Amazon.com Inc. or its affiliates. All Rights Reserved.
+// SPDX-License-Identifier: Apache-2.0
+// Do not modify this file. This file is machine generated, and any changes to it will be overwritten.
+package software.amazon.cryptography.dbencryptionsdk.dynamodb.json.model;
+
+import java.util.Objects;
+
+public class Json {
+
+  private final String utf8;
+
+  private final String text;
+
+  protected Json(BuilderImpl builder) {
+    this.utf8 = builder.utf8();
+    this.text = builder.text();
+  }
+
+  public String utf8() {
+    return this.utf8;
+  }
+
+  public String text() {
+    return this.text;
+  }
+
+  public Builder toBuilder() {
+    return new BuilderImpl(this);
+  }
+
+  public static Builder builder() {
+    return new BuilderImpl();
+  }
+
+  public interface Builder {
+    Builder utf8(String utf8);
+
+    String utf8();
+
+    Builder text(String text);
+
+    String text();
+
+    Json build();
+  }
+
+  static class BuilderImpl implements Builder {
+
+    protected String utf8;
+
+    protected String text;
+
+    protected BuilderImpl() {}
+
+    protected BuilderImpl(Json model) {
+      this.utf8 = model.utf8();
+      this.text = model.text();
+    }
+
+    public Builder utf8(String utf8) {
+      this.utf8 = utf8;
+      return this;
+    }
+
+    public String utf8() {
+      return this.utf8;
+    }
+
+    public Builder text(String text) {
+      this.text = text;
+      return this;
+    }
+
+    public String text() {
+      return this.text;
+    }
+
+    public Json build() {
+      if (!onlyOneNonNull()) {
+        throw new IllegalArgumentException(
+          "`Json` is a Union. A Union MUST have one and only one value set."
+        );
+      }
+      return new Json(this);
+    }
+
+    private boolean onlyOneNonNull() {
+      Object[] allValues = { this.utf8, this.text };
+      boolean haveOneNonNull = false;
+      for (Object o : allValues) {
+        if (Objects.nonNull(o)) {
+          if (haveOneNonNull) {
+            return false;
+          }
+          haveOneNonNull = true;
+        }
+      }
+      return haveOneNonNull;
+    }
+  }
+}
