DynamoDbEncryption/runtimes/net/Generated/JsonEncryptor/Actions.cs
@@ -9,8 +9,6 @@ namespace AWS.Cryptography.DbEncryptionSDK.DynamoDb.Json
   {
     private System.Collections.Generic.Dictionary<string, AWS.Cryptography.DbEncryptionSDK.StructuredEncryption.CryptoAction> _attributeActionsOnEncrypt;
     private System.Collections.Generic.Dictionary<string, AWS.Cryptography.DbEncryptionSDK.DynamoDb.Json.Actions> _nestedActionsOnEncrypt;
-    private System.Collections.Generic.Dictionary<string, AWS.Cryptography.DbEncryptionSDK.DynamoDb.Json.JsonEncryptorConfig> _nestedEncryptors;
-    private System.Collections.Generic.Dictionary<string, AWS.Cryptography.DbEncryptionSDK.DynamoDb.Json.KeyAccess> _eSDKActions;
     private AWS.Cryptography.DbEncryptionSDK.DynamoDb.Json.DefaultAction _defaultAction;
     public System.Collections.Generic.Dictionary<string, AWS.Cryptography.DbEncryptionSDK.StructuredEncryption.CryptoAction> AttributeActionsOnEncrypt
     {
@@ -29,24 +27,6 @@ namespace AWS.Cryptography.DbEncryptionSDK.DynamoDb.Json
     public bool IsSetNestedActionsOnEncrypt()
     {
       return this._nestedActionsOnEncrypt != null;
-    }
-    public System.Collections.Generic.Dictionary<string, AWS.Cryptography.DbEncryptionSDK.DynamoDb.Json.JsonEncryptorConfig> NestedEncryptors
-    {
-      get { return this._nestedEncryptors; }
-      set { this._nestedEncryptors = value; }
-    }
-    public bool IsSetNestedEncryptors()
-    {
-      return this._nestedEncryptors != null;
-    }
-    public System.Collections.Generic.Dictionary<string, AWS.Cryptography.DbEncryptionSDK.DynamoDb.Json.KeyAccess> ESDKActions
-    {
-      get { return this._eSDKActions; }
-      set { this._eSDKActions = value; }
-    }
-    public bool IsSetESDKActions()
-    {
-      return this._eSDKActions != null;
     }
     public AWS.Cryptography.DbEncryptionSDK.DynamoDb.Json.DefaultAction DefaultAction
     {
