DynamoDbEncryption/dafny/JsonEncryptor/src/foo.dfy
@@ -1,0 +1,35 @@
+include "Util.dfy"
+include "JsonToStruct.dfy"
+
+module Foo {
+
+  import opened StandardLibrary
+  import opened JsonEncryptorUtil
+  import opened AwsCryptographyDbEncryptionSdkDynamoDbJsonTypes
+  import CMP = AwsCryptographyMaterialProvidersTypes
+  import CSE = AwsCryptographyDbEncryptionSdkStructuredEncryptionTypes
+  import opened Wrappers
+  import JsonToStruct
+
+  datatype Config = Config(
+    nameonly logicalTableName : string,
+    nameonly cmpClient : CMP.IAwsCryptographicMaterialProvidersClient,
+    nameonly cmm: CMP.ICryptographicMaterialsManager,
+    nameonly attributeActionsOnEncrypt: AttributeActions,
+    nameonly allowedUnsignedAttributes: Option<seq<string>>,
+    nameonly allowedUnsignedAttributePrefix: Option<string>,
+    nameonly algorithmSuiteId: Option<CMP.DBEAlgorithmSuiteId>,
+    nameonly structuredEncryption: CSE.IStructuredEncryptionClient
+  )
+
+  type InternalConfig = Config
+
+  // method {:vcs_split_on_every_assert} EncryptObject2(config: InternalConfig, input: EncryptObjectInput)
+  method EncryptObject2(input: EncryptObjectInput)
+  {
+    //var origJson := JsonToStruct.SmithyJsonToObject(input.plaintextObject).MapFailure(e => E(e));
+    var origJson := JsonToStruct.SmithyJsonToObject(input.plaintextObject);
+    assert 3 == 3;
+  }
+
+}
